The answer is $\theta\left(p\right)=p\left(c\right)$ for some constant $c$. It is easy to check that this works, as \[\theta\left(p+1\right)=p\left(c\right)+1=\theta\left(p\right)+1\] and if $\theta\left(p\right)\neq0$, equivalently $p\left(c\right)\neq0$, then \[\theta\left(p\right)=p\left(c\right)\mid p\left(c\right)q\left(c\right)=\theta\left(p\cdot q\right).\] Now, let $\theta\left(x\right)=c$ and we prove that $\theta\left(p\right)=p\left(c\right)$ for all $p\in\mathbb{Z}\left[x\right]$ by induction on $\deg p$. First, we deal with constant. For $n\in\mathbb{Z}$, we have $\theta\left(n\right)=n+\theta\left(0\right)$ from $\theta\left(p+1\right)=\theta\left(p\right)+1$. Then \[n+\theta\left(0\right)=\theta\left(n\right)\mid\theta\left(2n\right)=2n+\theta\left(0\right),\] so \[n+\theta\left(0\right)\mid2\left(n+\theta\left(0\right)\right)-\left(2n+\theta\left(0\right)\right)=\theta\left(0\right),\] so $\theta\left(0\right)=0$, so $\theta\left(n\right)=n$. Now, we prove the claim for linear polynomials. For $n\in\mathbb{Z}$, observe that \[c+n=\theta\left(x\right)+n=\theta\left(x+n\right)\mid\theta\left(ax+an\right)=\theta\left(ax\right)+an,\] so \[c+n\mid\left(\theta\left(ax\right)+an\right)-a\left(c+n\right)=\theta\left(ax\right)-ac,\] so $\theta\left(ax\right)=ac$. Then $\theta\left(ax+b\right)=ac+b$ and the claim is true for linear $p$. Now, assume that $\theta\left(p\right)=p\left(c\right)$ whenever $\deg p\leq k$ for some constant $k$. Let $p$ be a polynomial of degree $k+1$. Then $\frac{p\left(x\right)-p\left(n\right)}{x-n}$ is a polynomial of degree $k$, so $\theta\left(\frac{p\left(x\right)-p\left(n\right)}{x-n}\right)=\frac{p\left(c\right)-p\left(n\right)}{c-n}$. Then \[\frac{p\left(c\right)-p\left(n\right)}{c-n}=\theta\left(\frac{p\left(x\right)-p\left(n\right)}{x-n}\right)\mid\theta\left(p\left(x\right)-p\left(n\right)\right)=\theta\left(p\right)-p\left(n\right),\] so \[\frac{p\left(c\right)-p\left(n\right)}{c-n}\mid\left(\theta\left(p\right)-p\left(n\right)\right)-\left(c-n\right)\left(\frac{p\left(c\right)-p\left(n\right)}{c-n}\right)=\theta\left(p\right)-p\left(c\right).\] As $\left|\frac{p\left(c\right)-p\left(n\right)}{c-n}\right|$ grows arbitrarily large as $n$ grows large, we have $\theta\left(p\right)=p\left(c\right)$, so the induction step is proven and hence the claim is true.