Observe that constant multiples of $x^2+3$ work; confirm by using the $x^3+y^3+z^3-3xyz$ identity.

First clear denominators so both sides are polynomials in $x,y,z$; by continuity we can now take $(x,y,z)=(x,-x,0)$ to deduce that $P$ is even. Now assume $P(t)=\displaystyle\sum_{k=0}^na_kt^k$ with $n$ even, $a_n\neq0$, and $a_{n-1}=0$. Substitute $(x,y,z)=(x,1,\frac{x+1}{2x-1})$ for $x\neq0,-1,\frac{1}{2}$ and multiply by $x(x+1)(2x-1)^n$ to get
\begin{align*}
&x(2x-1)^{n+1}P(x)+(2x-1)^{n+1}P(1)+(x+1)(2x-1)^nP(\frac{x+1}{2x-1})\\
=\quad&(x^2+x)(2x-1)^nP(x-1)+(x^2+x)(2x-1)^nP(\frac{x-2}{2x-1})\\&+(x^2+x)(2x-1)^nP(\frac{-2x^2+2x+1}{2x-1})
\end{align*}
where each term is a polynomial. Now we compute the $x^{2n+1}$ coefficient of each term.
\begin{itemize}
	\item Write
	\begin{align*}
		&x(2x-1)^{n+1}P(x)\\
		=&x(2^{n+1}x^{n+1}-(n+1)2^nx^n+O(x^{n-1}))(a_nx^n+O(x^{n-2}))\\
		=&2^{n+1}a_nx^{2n+2}-(n+1)2^na_nx^{2n+1}+O(x^{2n})
	\end{align*}
	so the coefficient in the first term is $-(n+1)2^na_n$.
	\item Write
	\begin{align*}
		&(x^2+x)(2x-1)^nP(x-1)\\
		=&(x^2+x)(2^nx^n-n2^{n-1}x^{n-1}+O(x^{n-2}))(a_n(x-1)^n+O(x^{n-2}))\\
		=&(x^2+x)(2^nx^n-n2^{n-1}x^{n-1}+O(x^{n-2}))(a_nx^n-na_nx^{n-1}+O(x^{n-2}))\\
		=&2^na_nx^{2n+2}+(2^na_n-n2^{n-1}a_n-n2^na_n)x^{2n+1}+O(x^{2n})
	\end{align*}
	so the coefficient in this term is $2^na_n-n2^{n-1}a_n-n2^na_n$.
	\item Write
	\begin{align*}
		&(x^2+x)(2x-1)^nP(\frac{-2x^2+2x+1}{2x-1})\\
		=&(x^2+x)\sum_{k=0}^na_k(-2x^2+2x+1)^k(2x-1)^{n-k}\\
		=&(x^2+x)(a_n(-2x^2+2x+1)^n+O(x^{2n-2}))\\
		=&(x^2+x)((-2)^na_nx^{2n}+2n(-2)^{n-1}a_nx^{2n-1}+O(x^{2n-2}))\\
		=&(-2)^na_nx^{2n+2}+((-2)^na_n+2n(-2)^{n-1}a_n)x^{2n+1}+O(x^{2n})
	\end{align*}
	so the coefficient here is $(-2)^na_n+2n(-2)^{n-1}a_n$.
	\item Observe that $(2x-1)^{n+1}P(1)$, $(x+1)(2x-1)^nP(\frac{x+1}{2x-1})=(x+1)\displaystyle\sum_{k=0}^na_k(x+1)^k(2x-1)^{n-k}$, and $(x^2+x)(2x-1)^nP(\frac{x-2}{2x-1})$ (expand the same way) are of degree less than $2n+1$, so there is no contribution here.
\end{itemize}
Now, the $x^{2n+1}$ coefficient on both sides of the equation above must be the same, since it is a polynomial identity which holds for infinitely many real $x$. Thus \[-(n+1)2^na_n=2^na_n-n2^{n-1}a_n-n2^na_n+(-2)^na_n+2n(-2)^{n-1}a_n.\] Using the fact that $a_n\neq0$ and $n$ is even, this reduces to $n=2$. So if $P$ is not the zero polynomial, then $P$ has degree $2$. We can quickly confirm that $cx^2+d$ works only when $d=3c$, giving us the solution claimed at the beginning.