Consider the $n-1$ distinct positive integers \[x_1<x_1+x_1<x_1+x_2<\cdots<x_1+x_{n-2}.\] Since $x_1+x_{n-2}<x_1+x_{n-1}=2n$, each of these are equal to $x_k$ for some index $k$. But the same is true of \[x_1<x_2<x_3<\cdots<x_{n-1},\] so each of these corresponding terms are equal. Then $x_1+x_i=x_{i+1}$ for $i=1,2,\ldots,n-2$. By induction, $x_i=jx_1$ for each index $i$, so $x_1=\frac{1}{n}\left(x_1+x_{n-1}\right)=2$ and hence $x_i=2i$ for each $i$. It is clear that this works as $x_i+x_{n-i}=2i+2\left(n-i\right)=2n$ and $x_i+x_j=x_{i+j}$ with $i+j<n$.