An equivalent condition is that $\frac{f\left(f\left(z\right)\right)-f\left(z\right)}{f\left(z\right)-z}$ is imaginary. We have
\begin{align*}
	\frac{f\left(f\left(z\right)\right)-f\left(z\right)}{f\left(z\right)-z}
	&=\frac{\left(z^2-19z\right)^2-20\left(z^2-19z\right)}{z^2-20z}\\
	&=\frac{\left(z^2-19z\right)\left(z^2-19z-20\right)}{z^2-20z}\\
	&=\left(z-19\right)\left(z+1\right)\\
	&=z^2-18z-19.
\end{align*}
Letting $z=a+11i$, we get $\left(a^2-18a-140\right)+\left(22a-198\right)i$ is imaginary, so $a^2-18a-140=0$. This implies $a=9\pm\sqrt{221}$, getting the answer $\boxed{230}$ as desired.