Let $n$ be a positive integer.  Given a sequence $\varepsilon_1$,  $\dots$,  $\varepsilon_{n - 1}$ with $\varepsilon_i = 0$ or $\varepsilon_i = 1$ for each $i = 1$,  $\dots$,  $n - 1$,  the sequences $a_0$,  $\dots$,  $a_n$ and $b_0$,  $\dots$,  $b_n$ are constructed by the following rules: \[a_0 = b_0 = 1, \quad a_1 = b_1 = 7,\] \[\begin{array}{lll}

	a_{i+1} = 

	\begin{cases}

		2a_{i-1} + 3a_i, \\

		3a_{i-1} + a_i, 

	\end{cases} & 

        \begin{array}{l} 

                \text{if } \varepsilon_i = 0, \\  

                \text{if } \varepsilon_i = 1, \end{array} 

         & \text{for each } i = 1, \dots, n - 1, \\[15pt]

        b_{i+1}= 

        \begin{cases}

		2b_{i-1} + 3b_i, \\

		3b_{i-1} + b_i, 

	\end{cases} & 

        \begin{array}{l} 

                \text{if } \varepsilon_{n-i} = 0, \\  

                \text{if } \varepsilon_{n-i} = 1, \end{array} 

         & \text{for each } i = 1, \dots, n - 1.

	\end{array}\]  Prove that $a_n = b_n$.
