Let $a_{i,j}$ be the integer in the $i$th row and $j$th column. Since $a_{i,j}\equiv1\pmod{n}$, we can write $a_{i,j}=nb_{i,j}+1$ for some integer $b_{i,j}$. Then \[n\sum_{j=1}^nb_{i,j}+n=\sum_{j=1}^na_{i,j}\equiv n\pmod{n^2},\] so $n$ divides $\displaystyle\sum_{j=1}^nb_{i,j}$. Similarly, $n$ divides $\displaystyle\sum_{i=1}^nb_{i,j}$. So let us define $c_i=\frac{1}{n}\displaystyle\sum_{j=1}^nb_{i,j}$, an integer.

First, observe that
\begin{align*}
	R_i&=\prod_{j=1}^n(nb_{i,j}+1)\\
	&\equiv1+n\sum_{j=1}^nb_{i,j}+n^2\sum_{1\leq j_1<j_2\leq n}b_{i,j_1}b_{i,j_2}+n^3\sum_{1\leq j_1<j_2<j_3\leq n}b_{i,j_1}b_{i,j_2}b_{i,j_3}\pmod{n^4}
\end{align*}
because the remaining part of the expansion has a factor of $n^4$. Next, we appeal to Newton's identities to see that \[\sum_{1\leq j_1<j_2\leq n}b_{i,j_1}b_{i,j_2}=\frac{1}{2}\left(\sum_{j=1}^nb_{i,j}\right)^2-\frac{1}{2}\sum_{j=1}^nb_{i,j}^2\] and \[\sum_{1\leq j_1<j_2<j_3\leq n}b_{i,j_1}b_{i,j_2}b_{i,j_3}=\frac{1}{6}\left(\sum_{j=1}^nb_{i,j}\right)^3-\frac{1}{2}\sum_{j=1}^nb_{i,j}\sum_{j=1}^nb_{i,j}^2+\frac{1}{3}\sum_{j=1}^nb_{i,j}^3.\] Before we move on, note that $\frac{n}{2},\frac{n}{3},\frac{n}{6}$ each make sense modulo $n^4$. This is because if $p$ divides both $n^4$ and the denominator of one of these fractions, then $p$ divides $n$ too and thus it is a non-issue. With this in mind, we can write
\begin{align*}
	n^2\sum_{1\leq j_1<j_2\leq n}b_{i,j_1}b_{i,j_2}&=\frac{n^2}{2}\left(\sum_{j=1}^nb_{i,j}\right)^2-\frac{n^2}{2}\sum_{i=1}^nb_{i,j}^2\\
	&=\frac{n^4c_i^2}{2}-\frac{n^2}{2}\sum_{j=1}^nb_{i,j}^2\\
	&\equiv\frac{n^4c_i}{2}-\frac{n^2}{2}\sum_{j=1}^nb_{i,j}^2\pmod{n^4}\\
	&\equiv\frac{n^3}{2}\sum_{j=1}^nb_{i,j}-\frac{n^2}{2}\sum_{j=1}^nb_{i,j}^2\pmod{n^4}
\end{align*}
where the congruence comes from the fact that $\frac{1}{n^4}\cdot\frac{n^4c_i^2-n^4c_i}{2}=\frac{c_i(c_i-1)}{2}$ is an integer. Similarly,
\begin{align*}
	n^3\sum_{1\leq j_1<j_2<j_3\leq n}b_{i,j_1}b_{i,j_2}b_{i,j_3}&=\frac{n^3}{6}\left(\sum_{j=1}^nb_{i,j}\right)^3-\frac{n^3}{2}\sum_{j=1}^nb_{i,j}\sum_{j=1}^nb_{i,j}^2+\frac{n^3}{3}\sum_{j=1}^nb_{i,j}^3\\
	&=\frac{n^6c_i^3}{6}-\frac{n^4c_i}{2}\left[\left(\sum_{j=1}^nb_{i,j}\right)^2-2\sum_{1\leq j_1<j_2\leq n}b_{i,j_1}b_{i,j_2}\right]+\frac{n^3}{3}\sum_{j=1}^nb_{i,j}^3\\
	&=\frac{n^6c_i^3}{6}-\frac{n^6c_i^3}{2}+n^4c_i\sum_{1\leq j_1<j_2\leq n}b_{i,j_2}b_{i,j_1}+\frac{n^3}{3}\sum_{j=1}^nb_{i,j}^3\\
	&=-n^4\cdot\frac{n^2c_i^3}{3}+n^4c_i\sum_{1\leq j_1<j_2\leq n}b_{i,j_1}b_{i,j_2}+\frac{n^3}{3}\sum_{j=1}^nb_{i,j}^3\\
	&\equiv\frac{n^3}{3}\sum_{j=1}^nb_{i,j}^3\pmod{n^4}
\end{align*}
where we used Newton's identity again.

Thus \[R_i\equiv 1+n\sum_{j=1}^nb_{i,j}+\frac{n^3}{2}\sum_{j=1}^nb_{i,j}-\frac{n^2}{2}\sum_{j=1}^nb_{i,j}^2+\frac{n^3}{3}\sum_{j=1}^nb_{i,j}^3\pmod{n^4}\] so
\begin{align*}
	R_1+\cdots+R_n&\equiv\sum_{i=1}^n1+n\sum_{j=1}^nb_{i,j}+\frac{n^3}{2}\sum_{j=1}^nb_{i,j}-\frac{n^2}{2}\sum_{j=1}^nb_{i,j}^2+\frac{n^3}{3}\sum_{j=1}^nb_{i,j}^3\pmod{n^4}\\
	&\equiv n+\left(n+\frac{n^3}{2}\right)\sum_{1\leq i,j\leq n}b_{i,j}-\frac{n^2}{2}\sum_{1\leq i,j\leq n}b_{i,j}^2+\frac{n^3}{3}\sum_{1\leq i,j\leq n}b_{i,j}^3\pmod{n^4}
\end{align*}
which is symmetrical and $i$ and $j$. It follows that \[R_1+\cdots+R_n\equiv C_1+\cdots+C_n\pmod{n^4}\] as desired.