It suffices to prove that $\frac{1}{p}-2S_q\equiv1\pmod p$. Write
\begin{align*}
	2S_q&=\displaystyle\sum_{k=1}^{\frac{p-1}{2}}\frac{2}{(3k-1)\cdot3k\cdot(3k+1)}\\
	&=\displaystyle\sum_{k=1}^{\frac{p-1}{2}}\frac{1}{3k-1}-\frac{2}{3k}+\frac{1}{3k+1}\\
	&=\displaystyle\sum_{k=1}^{\frac{p-1}{2}}\frac{1}{3k-1}+\frac{1}{3k}+\frac{1}{3k+1}-\displaystyle\sum_{k=1}^{\frac{p-1}{2}}\frac{1}{k}\\
	&=-1+\displaystyle\sum_{k=\frac{p+1}{2}}^{\frac{3p-1}{2}}\frac{1}{k}.
\end{align*}
Thus
\begin{align*}
	\frac{1}{p}-2S_q-1&=-\displaystyle\sum_{k=\frac{p+1}{2}}^{p-1}\frac{1}{k}-\displaystyle\sum_{k=p+1}^{\frac{3p-1}{2}}\frac{1}{k}\\
	&\equiv-\displaystyle\sum_{k=\frac{p+1}{2}}^{p-1}\frac{1}{k}-\displaystyle\sum_{k=1}^{\frac{p-1}{2}}\frac{1}{k}\pmod p\\
	&\equiv\displaystyle\sum_{k=1}^{\frac{p-1}{2}}\frac{1}{k}-\displaystyle\sum_{k=1}^{\frac{p-1}{2}}\frac{1}{k}\pmod p\\
	&\equiv0\pmod p
\end{align*}
as desired.