Seja $\phi: \NN \to \NN$ a bijeção tal que $\phi(1) = 1$ e, para todo $k \in \NN$, temos $\phi(k^2 + 2r - 1) = k^2 + k + r$, para $r$ inteiro com $1 \le r \le k+1$ e $\phi(k^2 + 2r) = k^2 + k + 1 - r$, para $r$ inteiro com $1 \le r \le k$.

Assim, por exemplo, $\phi(1) = 1, \phi(2) = 3, \phi(3) = 2, \phi(4) = 4, \phi(5) = 7, \phi(6) = 6, \phi(7) = 8, \phi(8) = 5, \phi(9) = 9$.

\begin{enumerate}[label = (\alph*)]
	\item Prove que se $(a_n)$ é uma sequência tal que $\sum a_n$ converge então $\sum a_{\phi(n)}$ converge e $\sum a_n = \sum a_{\phi(n)}$.
	\item Exiba uma sequência $(b_n)$ tal que $\sum b_n$ diverge mas $\sum b_{\phi(n)}$ converge.
\end{enumerate}
