Let $\left\{F_n\right\}$ be the Fibonacci sequence satisfying $F_1=F_2=1$ and $F_n=F_{n-1}+F_{n-2}$ for all integers $n$. Let $\left\{T_n\left(x\right)\right\}$ be the Tchebyshev polynomials satisfying $T_0\left(x\right)=1$, $T_1\left(x\right)=x$, and $T_n\left(x\right)=2xT_{n-1}\left(x\right)-T_{n-1}\left(x\right)$ for all integers $n\geq2$. It is well-known that $T_n\left(\cos\theta\right)=\cos n\theta$ is an identity for the complex function $\cos$.

\begin{solutionlemma}
$x_n=T_{F_n}\left(a\right)$ for all non-negative integers $n$.
\end{solutionlemma}
\begin{lemmaproof}
We prove this by strong induction on $n$. The base cases of $n=0,1,2,3$ are true as $x_0=1,x_1=a,x_2=a$, and \[x_3=2\cdot a\cdot a-1=2a^2-1=T_2\left(a\right).\] Now, assume that this equality holds for $n=0,1,\ldots,m$ for some integer $m\geq3$. We prove that it holds for $n=m+1$.

First note that
\begin{align*}
	\cos\left(F_{m+1}\theta\right)+\cos\left(F_{m-2}\theta\right)&=\cos\left(F_m\theta+F_{m-1}\theta\right)+\cos\left(F_m\theta-F_{m-1}\theta\right)\\
	&=\left(\cos\left(F_m\theta\right)\cos\left(F_{m-1}\theta\right)-\sin\left(F_m\theta\right)\sin\left(F_{m-1}\theta\right)\right)\\&+\left(\cos\left(F_m\theta\right)\cos\left(F_{m-1}\theta\right)+\sin\left(F_m\theta\right)\sin\left(F_{m-1}\theta\right)\right)\\
	&=2\cos\left(F_m\theta\right)\cos\left(F_{m-1}\theta\right).
\end{align*}
Letting $\theta=\arccos a$, we have
\begin{align*}
	x_{m+1}&=2x_mx_{m-1}-x_{m-2}\\
	&=2T_{F_m}\left(a\right)T_{F_{m-1}}\left(a\right)-T_{F_{m-2}}\left(a\right)\\
	&=2\cos\left(F_m\theta\right)\cos\left(F_{m-1}\theta\right)-\cos\left(F_{m-2}\theta\right)\\
	&=\cos\left(F_{m+1}\theta\right)\\
	&=T_{F_{m+1}}\left(a\right)
\end{align*}
so the inductive step is proven and hence the lemma is true.
\end{lemmaproof}

Suppose that $x_r=0$ for some $r$. Let $\theta=\arccos a$. Then $T_{F_r}\left(a\right)=0$, so $\cos\left(F_r\theta\right)=0$ and thus $F_r\theta=\frac{\pi}{2}+\pi k$ for some integer $k$. Then $\theta=\frac{\pi\left(2k+1\right)}{2F_r}$ for some integer $k$.

Now, consider the sequence $\left\{G_n\right\}$ such that $G_n$ is the remainder when $F_n$ is divided by $4F_r$. Since there are only finitely many remainders when dividing by $4F_r$ but there are infinitely many terms of $\left\{G_n\right\}$, the Pigeonhole Principle on pairs $\left(G_n,G_{n-1}\right)$ tells us that there are integers $b<c$ such that $F_b$ and $F_c$ leave the same remainder and $F_{b+1}$ and $F_{c+1}$ leave the same remainder.

Let $d=c-b$. I claim that $F_{m+d}\equiv F_m\pmod{4F_r}$ for all integers $m$. First, we prove this for all integers $m\geq b$. We do this by strong induction on $m$. The base cases of $m=b,b+1$ are true by definition of $b,c$. Now, suppose that this is true for $m=b,b+1,\ldots,b+j$ for some positive integer $j$. Then \[F_{m+j+1+d}=F_{m+j+d}+F_{m+j-1+d}\equiv F_{m+j}+F_{m+j-1}\equiv F_{m+j+1}\pmod{4F_r},\] so this is true for $j+1$ and hence by induction this is true for $m\geq b$. Next, we prove this for all integers $m\leq b+1$. We do this by strong induction on $m$. The base cases of $m=b+1,b$ are true from above. Now, suppose that this is true for $m=b+1,b,\ldots,b-j$ for some non-negative integer $j$. Then \[F_{m+b-j-1+d}=F_{m+b-j+1+d}-F_{m+b-j+d}\equiv F_{m+b-j+1}-F_{m+b-j}\equiv F_{m+b-j-1}\pmod{4F_r},\] so this is true for $j+1$ and hence by induction this is true for $m\leq b+1$. Thus there is a positive integer $d$ such that $F_{m+d}\equiv F_m\pmod{4F_n}$ for all integers $m$.

Let $m$ be a non-negative integer and let $F_{m+d}-F_m=4F_n\ell$ for some integer $\ell$. Then
\begin{align*}
	x_{m+d}&=T_{F_{m+d}}\left(a\right)\\
	&=\cos\left(F_{m+d}\theta\right)\\
	&=\cos\left(\frac{F_{m+d}\pi\left(2k+1\right)}{2F_n}\right)\\
	&=\cos\left(\frac{F_m\pi\left(2k+1\right)}{2F_n}+2\pi\left(2k+1\right)\ell\right)\\
	&=\cos\left(\frac{F_m\pi\left(2k+1\right)}{2F_n}\right)\\
	&=\cos\left(F_m\theta\right)\\
	&=T_{F_m}\left(a\right)\\
	&=x_m
\end{align*}
so the sequence is periodic.