Let $M$ be the numerator and $N$ be the denominator of the expression. Then the problem is equivalent to $N$ dividing $M-N=\left(p+q\right)^{p-q}\left(p-q\right)^{p-q}\left(\left(p+q\right)^{2q}-\left(p-q\right)^{2q}\right)$. But clearly $N$ is relatively prime to $\left(p+q\right)\left(p-q\right)$, so $N$ divides $\left(p+q\right)^{2q}-\left(p-q\right)^{2q}$.

First, suppose that $q>3$. Let $r$ be a prime divisor of $N$, clearly $r$ is odd since $N$ is odd. Observe that \[N\equiv q^{2p}-1\equiv q^2-1\pmod p,\] so if $r=p$, then $p$ divides $q-1$ or $q+1$. But $q+1<p$, contradiction. So $r\neq p$.

Let $d=\ord_r\left(\frac{p+q}{p-q}\right)\mid 2q$. If $d=1$, then $r=q$. If $d=2$, then $r\mid4pq$, but $r\neq2,p$ so $r=q$. If $d=q$ or $2q$, then $r\equiv1\pmod q$. Thus, either $r=q$ or $r\equiv1\pmod q$, so all factors of $N$ are $0,1\pmod q$.

Next, observe that $N\equiv p^{2p}-1\pmod q$, so $p^p-1$ and $p^p+1$ are $0,1\pmod q$. Clearly $p^p+1\not\equiv1\pmod q$, so $p^p+1\equiv0\pmod q$. Then $p^p-1\equiv-2\pmod q$, so either $q=2$ or $q=3$, contradiction. Thus, $q\leq3$.

Now, observe that \[\left(p+q\right)^{p-1}\left(p-q\right)^{p+q}-1=N\leq\left(p+q\right)^{2q}-\left(p-q\right)^{2q}\] since the right hand side is positive. If $p>3q$, then $\left(p+q\right)^{p-q}\left(p-q\right)^{p+q}>\left(p+q\right)^{2q}$ but $1\leq\left(p-q\right)^{2q}$, so this inequality is false. Thus, $p\leq3q$. Thus, the only possibilities are $\left(3,2\right),\left(5,2\right),\left(5,3\right),\left(7,3\right)$. We also have the condition that $\left(p-q\right)^{p+q}\leq\left(p+q\right)^{3q-p}$ otherwise the inequality still fails. Checking each of these cases, we see that the only remaining cases to check are $\left(3,2\right)$ and $\left(5,3\right)$. These give that $\frac{\left(p+q\right)^{2q}-\left(p-q\right)^{2q}}{N}$ is $\frac{5^4-1}{4}$ and $\frac{8^6-2^6}{2^{14}-1}$, respectively. The former is an integer but the latter is not because it is $\frac{2^6\left(2^{12}-1\right)}{2^{14}-1}$. Thus, the only solution is $\left(p,q\right)=\boxed{\left(3,2\right)}$.