By the Coaxial Lemma, \[\frac{XF}{XE}=\frac{XF\cdot XP}{XE\cdot XP}=\frac{DF'\cdot DP}{DE'\cdot DP}=\frac{DF'}{DE'}.\] Let $M'$ be the midpoint of $EF$, $D'=EF\cap BC$. Observe that $MM'$ is parallel to the $A$-angle bisector. Then
\begin{align*}
\left(E,F;X,D'\right)&=\frac{XE}{XF}\div\frac{D'E}{D'F}=-\frac{XE}{XF}\cdot\frac{M'E}{M'F}\div\frac{D'E}{D'F}\\
&=-\frac{XE}{XF}\left(E,F;M',D'\right)\stackrel{M}{=}-\frac{XE}{XF}\left(E',F';\infty_{AI},D\right)\\
&=-\frac{XE}{XF}\cdot\frac{\infty_{AI}E'}{\infty_{AI}F'}\div\frac{DE'}{DF'}=-\frac{XE}{XF}\cdot\frac{DF'}{DE'}=-1,
\end{align*}
so $AX$ is the $A$-Nagel line. Then $\frac{FX}{XE}=\frac{CA}{AB}$, so \[FE=\sqrt{FA^2+EA^2-2FA\cdot EA\cos\angle{A}}=\sqrt{4^2+6^2-2\cdot4\cdot6\cdot\frac{13}{15}}=\frac{2\sqrt{65}}{5},\] so \[\left|XE-XF\right|=\left|\frac{9}{19}\cdot\frac{2\sqrt{65}}{5}-\frac{10}{19}\cdot\frac{2\sqrt{65}}{5}\right|=\boxed{\frac{2\sqrt{65}}{95}}.\]